src/program_logic/crash_adequacy.v
@@ -2,14 +2,18 @@ From iris.proofmode Require Import tactics.
 From iris.algebra Require Import gmap auth agree gset coPset.
 From Perennial.base_logic.lib Require Import wsat.
 From Perennial.program_logic Require Export weakestpre.
-From Perennial.program_logic Require Export step_fupd_extra crash_lang crash_weakestpre.
-Import uPred.
-Import language.
+From Perennial.program_logic Require Export step_fupd_extra language crash_lang.
 
 Set Default Proof Using "Type".
 
+From self.program_logic Require Export crash_weakestpre.
+(* From Perennial.program_logic Require Export language. *)
+
+Import uPred.
+Import language.
+
 Section crash_adequacy.
-Context `{!irisGS Λ Σ, generationGS Λ Σ}.
+Context `{!irisGS Λ Σ}.
 Implicit Types s : stuckness.
 Implicit Types e : expr Λ.
 Implicit Types P Q : iProp Σ.
@@ -32,20 +36,19 @@ Lemma wpc_step s e1 σ1 g1 ns D κ κs e2 σ2 g2 efs m Φ Φc :
   prim_step e1 σ1 g1 κ e2 σ2 g2 efs →
   state_interp σ1 m -∗
   global_state_interp g1 ns mj D (κ ++ κs) -∗
-  WPC e1 @ s; ⊤ {{ Φ }} {{ Φc }} -∗ NC 1 -∗
+  WPC e1 @ s; ⊤ {{ Φ }} {{ Φc }} -∗
   £ (S $ num_laters_per_step ns) -∗
   ||={⊤|⊤,∅|∅}=> ||▷=>^(S $ num_laters_per_step ns) ||={∅|∅,⊤|⊤}=>
   state_interp σ2 (length efs + m) ∗
   global_state_interp g2 (step_count_next ns) mj D κs ∗
   WPC e2 @ s; ⊤ {{ Φ }} {{ Φc }} ∗
-  wptp s efs ∗
-  NC 1.
+  wptp s efs.
 Proof.
-  rewrite {1}wpc0_unfold /wpc_pre. iIntros (?) "Hσ Hg H HNC Hlc".
+  rewrite {1}wpc0_unfold /wpc_pre. iIntros (?) "Hσ Hg H Hlc".
   rewrite (val_stuck e1 σ1 g1 κ e2 σ2 g2 efs) //.
   iDestruct "H" as "(H&_)".
   iMod (fupd2_mask_subseteq ⊤ (⊤ ∖ D)) as "Hclo"; try set_solver+.
-  iMod ("H" $! _ σ1 with "Hσ Hg HNC Hlc") as "H".
+  iMod ("H" $! σ1 with "Hσ Hg Hlc") as "H".
   iModIntro.
   iApply (step_fupd2N_wand with "H"). iIntros "(_&H)".
   iMod ("H" $! e2 σ2 g2 efs with "[//]") as "H".
@@ -57,23 +60,23 @@ Lemma wptp_step s e1 t1 t2 κ κs σ1 g1 ns D σ2 g2 Φ Φc :
   step (e1 :: t1,(σ1,g1)) κ (t2, (σ2,g2)) →
   state_interp σ1 (length t1) -∗
   global_state_interp g1 ns mj D (κ ++ κs) -∗
-  WPC e1 @ s; ⊤ {{ Φ }} {{ Φc }}-∗ wptp s t1 -∗ NC 1 -∗
+  WPC e1 @ s; ⊤ {{ Φ }} {{ Φc }}-∗ wptp s t1 -∗
   £ (S $ num_laters_per_step ns) ==∗
   ∃ e2 t2', ⌜t2 = e2 :: t2'⌝ ∗
   ||={⊤|⊤,∅|∅}=> ||▷=>^(S $ num_laters_per_step ns) ||={∅|∅,⊤|⊤}=>
   state_interp σ2 (pred (length t2)) ∗
   global_state_interp g2 (step_count_next ns) mj D κs ∗
-  WPC e2 @ s; ⊤ {{ Φ }} {{ Φc}} ∗ wptp s t2' ∗ NC 1.
+  WPC e2 @ s; ⊤ {{ Φ }} {{ Φc}} ∗ wptp s t2'.
 Proof.
-  iIntros (Hstep) "Hσ Hg He Ht HNC Hlc".
+  iIntros (Hstep) "Hσ Hg He Ht Hlc".
   destruct Hstep as [e1' σ1' g1' e2' σ2' g2' efs [|? t1'] t2' ?? Hstep]; simplify_eq/=.
   - iExists e2', (t2' ++ efs). iModIntro. iSplitR; first by eauto.
-    iMod (wpc_step with "Hσ Hg He HNC Hlc") as "H"; first done. iModIntro.
+    iMod (wpc_step with "Hσ Hg He Hlc") as "H"; first done. iModIntro.
     iApply (step_fupd2N_wand with "H"). iIntros ">(Hσ & Hg & He2 & Hefs) !>".
     rewrite Nat.add_comm app_length. by iFrame.
   - iExists e, (t1' ++ e2' :: t2' ++ efs); iSplitR; first eauto.
     iDestruct "Ht" as "(Ht1 & He1 & Ht2)".
-    iModIntro. iMod (wpc_step with "Hσ Hg He1 HNC Hlc") as "H"; first done. iModIntro.
+    iModIntro. iMod (wpc_step with "Hσ Hg He1 Hlc") as "H"; first done. iModIntro.
     iApply (step_fupd2N_wand with "H"). iIntros ">(Hσ & Hg & He2 & Hefs) !>".
     rewrite !app_length /= !app_length.
     replace (length t1' + S (length t2' + length efs))
@@ -105,52 +108,51 @@ Proof.
     rewrite -Nat.iter_succ_r /=. lia.
 Qed.
 
-Lemma wptp_steps s n e1 t1 κs κs' t2 σ1 g1 ns D σ2 g2 Φ Φc :
+Lemma wptp_steps s (n : nat) e1 t1 κs κs' t2 σ1 g1 ns D σ2 g2 Φ Φc :
   nsteps n (e1 :: t1, (σ1,g1)) κs (t2, (σ2,g2)) →
   state_interp σ1 (length t1) -∗
   global_state_interp g1 ns mj D (κs ++ κs') -∗
-  WPC e1 @ s; ⊤ {{ Φ }} {{ Φc }} -∗ wptp s t1 -∗ NC 1 -∗
+  WPC e1 @ s; ⊤ {{ Φ }} {{ Φc }} -∗ wptp s t1 -∗
   £ (steps_sum num_laters_per_step step_count_next ns n) -∗
   (||={⊤|⊤, ∅|∅}=> ||▷=>^(steps_sum num_laters_per_step step_count_next ns n) ||={∅|∅,⊤|⊤}=> ∃ e2 t2',
     ⌜t2 = e2 :: t2'⌝ ∗
     state_interp σ2 (pred (length t2)) ∗
     global_state_interp g2 (Nat.iter n step_count_next ns) mj D κs' ∗
-    WPC e2 @ s; ⊤ {{ Φ }} {{ Φc }} ∗ wptp s t2' ∗
-    NC 1).
+    WPC e2 @ s; ⊤ {{ Φ }} {{ Φc }} ∗ wptp s t2').
 Proof.
   revert e1 t1 κs κs' t2 σ1 g1 ns σ2 g2; simpl.
   induction n as [|n IH]=> e1 t1 κs κs' t2 σ1 g1 ns σ2 g2 /=.
-  { inversion_clear 1; iIntros "??????"; iExists e1, t1; iFrame; eauto 10.
+  { inversion_clear 1; iIntros "?????"; iExists e1, t1; iFrame; eauto 10.
     iApply fupd2_mask_intro_subseteq; eauto. }
-  iIntros (Hsteps) "Hσ Hg He Ht HNC Hlc". inversion_clear Hsteps as [|?? [t1' [σ1' g1']]].
+  iIntros (Hsteps) "Hσ Hg He Ht Hlc". inversion_clear Hsteps as [|?? [t1' [σ1' g1']]].
   rewrite -(assoc_L (++)).
   rewrite -Nat.add_succ_l lc_split.
   iDestruct "Hlc" as "[Hlc1 Hlc2]".
   iApply step_fupd2N_inner_add.
-  iMod (wptp_step with "Hσ Hg He Ht HNC Hlc1") as (e1' t1'' ?) ">H"; first eauto; simplify_eq.
+  iMod (wptp_step with "Hσ Hg He Ht Hlc1") as (e1' t1'' ?) ">H"; first eauto; simplify_eq.
   iApply (step_fupd2N_wand with "H"). iIntros "!> H".
   iMod "H".
-  iDestruct "H" as "(Hσ & Hg & He & Ht & HNC)".
-  iMod (IH with "Hσ Hg He Ht HNC Hlc2") as "IH"; first done.
+  iDestruct "H" as "(Hσ & Hg & He & Ht)".
+  iMod (IH with "Hσ Hg He Ht Hlc2") as "IH"; first done.
   rewrite -Nat.iter_succ_r.
   iModIntro. iModIntro. eauto.
 Qed.
 
-Lemma wpc_safe κs m e σ g ns D Φ Φc q :
+Lemma wpc_safe κs m e σ g ns D Φ Φc :
   state_interp σ m -∗
   global_state_interp g ns mj D κs -∗
-  WPC e @ ⊤ {{ Φ }} {{ Φc }} -∗ NC q -∗
+  WPC e @ ⊤ {{ Φ }} {{ Φc }} -∗
   £ (S $ num_laters_per_step ns) -∗
   ||={⊤|⊤, ∅|∅}=> ||▷=>^(num_laters_per_step ns + 1)
   ⌜is_Some (to_val e) ∨ reducible e σ g⌝.
 Proof.
   rewrite wpc0_unfold /wpc_pre. iIntros "Hσ Hg H". iDestruct "H" as "(H&_)".
   destruct (to_val e) as [v|] eqn:?.
-  { iIntros "_ _". iApply fupd2_mask_intro; [done..|].
+  { iIntros "_". iApply fupd2_mask_intro; [done..|].
     iIntros "_". iApply step_fupd2N_later. auto. }
-  iIntros "HNC Hlc".
+  iIntros "Hlc".
   iMod (fupd2_mask_subseteq ⊤ (⊤ ∖ D)) as "Hclo"; try set_solver+.
-  iMod ("H" $! _ _ _ _ _ [] with "[$] [$] [$] [$]") as "H".
+  iMod ("H" $! _ _ _ _ [] with "[$] [$] [$]") as "H".
   simpl. iModIntro. rewrite [_ + 1]comm. iApply (step_fupd2N_wand with "H").
   iNext. iIntros "(%Hred&Hclo')". eauto.
 Qed.
@@ -161,31 +163,29 @@ Local Lemma wptp0_strong_adequacy Φ Φc κs' s n e1 t1 κs t2 σ1 g1 ns D σ2 g
   global_state_interp g1 ns mj D (κs ++ κs') -∗
   WPC e1 @ s; ⊤ {{ Φ }} {{ Φc }} -∗
   wptp s t1 -∗
-  NC 1 -∗
   £ (steps_sum num_laters_per_step step_count_next ns n) -∗
   ||={⊤|⊤,∅|∅}=> ||▷=>^(steps_sum num_laters_per_step step_count_next ns n) ||={∅|∅, ⊤|⊤}=> (∃ e2 t2',
     ⌜ t2 = e2 :: t2' ⌝ ∗
     state_interp σ2 (length t2') ∗
     global_state_interp g2 (Nat.iter n step_count_next ns) mj D κs' ∗
     from_option Φ True (to_val e2) ∗
-    ([∗ list] v ∈ omap to_val t2', fork_post v) ∗
-    NC 1).
+    ([∗ list] v ∈ omap to_val t2', fork_post v)).
 Proof.
-  iIntros (Hstep) "Hσ Hg He Ht HNC Hlc".
-  iMod (wptp_steps with "Hσ Hg He Ht HNC Hlc") as "Hwp"; first done.
+  iIntros (Hstep) "Hσ Hg He Ht Hlc".
+  iMod (wptp_steps with "Hσ Hg He Ht Hlc") as "Hwp"; first done.
   iModIntro. iApply (step_fupd2N_wand with "Hwp").
-  iMod 1 as (e2' t2' ?) "(Hσ & Hg & Hwp & Ht & HNC)"; simplify_eq/=.
+  iMod 1 as (e2' t2' ?) "(Hσ & Hg & Hwp & Ht)"; simplify_eq/=.
   iExists _, _. iSplitL ""; first done. iFrame "Hσ".
   iMod (fupd2_mask_subseteq ⊤ (⊤ ∖ D)) as "Hclo"; try set_solver+.
-  iMod (wpc0_value_inv_option with "Hwp Hg HNC") as "($&Hg&HNC)".
+  iMod (wpc0_value_inv_option with "Hwp Hg") as "[$ Hg]".
   clear Hstep. iMod "Hclo" as "_". iInduction t2' as [|e t2'] "IH"; csimpl; first by iFrame.
   iDestruct "Ht" as "[Hv Ht]".
   destruct (to_val e) as [v|] eqn:He.
   + apply of_to_val in He as <-.
     iMod (fupd2_mask_subseteq ⊤ (⊤ ∖ D)) as "Hclo'"; try set_solver+.
-    iMod (wpc0_value_inv' with "Hv Hg HNC") as "($&?&?)".
+    iMod (wpc0_value_inv' with "Hv Hg") as "($ & ?)".
     iMod "Hclo'" as "_".
-    by iApply ("IH" with "[$] [$] [$]").
+    by iApply ("IH" with "[$] [$]").
   + by iApply ("IH" with "[$] [$]").
 Qed.
 
@@ -196,23 +196,22 @@ Local Lemma wptp0_progress Φ Φc κs' n e1 t1 κs t2 σ1 g1 ns D σ2 g2 e2 :
   global_state_interp g1 ns mj D (κs ++ κs') -∗
   WPC e1 @ NotStuck; ⊤ {{ Φ }} {{ Φc }} -∗
   wptp NotStuck t1 -∗
-  NC 1 -∗
   £ (steps_sum num_laters_per_step step_count_next ns (S n)) -∗
   ||={⊤|⊤,∅|∅}=> ||▷=>^(steps_sum num_laters_per_step step_count_next ns n) ||={∅|∅, ∅|∅}=>
   ||▷=>^(num_laters_per_step (Nat.iter n step_count_next ns) + 1)
    ⌜ not_stuck e2 σ2 g2 ⌝.
 Proof.
-  iIntros (Hstep Hel) "Hσ Hg He Ht HNC Hlc".
+  iIntros (Hstep Hel) "Hσ Hg He Ht Hlc".
   rewrite steps_sum_S_r.
   iDestruct "Hlc" as "[Hlc1 Hlc2]".
-  iMod (wptp_steps with "Hσ Hg He Ht HNC Hlc1") as "Hwp"; first done.
+  iMod (wptp_steps with "Hσ Hg He Ht Hlc1") as "Hwp"; first done.
   iModIntro. iApply (step_fupd2N_wand with "Hwp").
-  iMod 1 as (e2' t2' ?) "(Hσ & Hg & Hwp & Ht & HNC)"; simplify_eq/=.
+  iMod 1 as (e2' t2' ?) "(Hσ & Hg & Hwp & Ht)"; simplify_eq/=.
   apply elem_of_cons in Hel as [<-|(t1''&t2''&->)%elem_of_list_split].
-  - iPoseProof (wpc_safe with "Hσ Hg Hwp HNC Hlc2") as "H".
+  - iPoseProof (wpc_safe with "Hσ Hg Hwp Hlc2") as "H".
     iMod "H". eauto.
   - iDestruct "Ht" as "(_ & He' & _)".
-    iPoseProof (wpc_safe with "Hσ Hg He' HNC Hlc2") as "H".
+    iPoseProof (wpc_safe with "Hσ Hg He' Hlc2") as "H".
     by iMod "H".
 Qed.
 
@@ -222,34 +221,33 @@ Local Lemma wptp0_strong_crash_adequacy Φ Φc κs' s n e1 t1 κs t2 σ1 g1 ns D
   global_state_interp g1 ns mj D (κs ++ κs') -∗
   WPC e1 @ s; ⊤ {{ Φ }} {{ Φc }} -∗
   wptp s t1 -∗
-  NC 1 -∗
   £ (steps_sum num_laters_per_step step_count_next ns (S n)) -∗
   ||={⊤|⊤,∅|∅}=> ||▷=>^(steps_sum num_laters_per_step step_count_next ns (S n)) ||={∅|∅, ⊤|⊤}=>
   ▷ (∃ e2 t2',
     ⌜ t2 = e2 :: t2' ⌝ ∗
-    Φc ∗ state_interp σ2 (length t2') ∗ global_state_interp g2 ((Nat.iter n step_count_next ns)) mj D κs' ∗ C).
+    Φc ∗ state_interp σ2 (length t2') ∗ global_state_interp g2 ((Nat.iter n step_count_next ns)) mj D κs').
 Proof.
-  iIntros (Hstep) "Hσ Hg He Ht HNC Hlc".
+  iIntros (Hstep) "Hσ Hg He Ht Hlc".
   rewrite steps_sum_S_r.
   iDestruct "Hlc" as "[Hlc1 Hlc2]".
-  iDestruct (wptp_steps with "Hσ Hg He Ht HNC Hlc1") as "Hwp"; first done.
+  iDestruct (wptp_steps with "Hσ Hg He Ht Hlc1") as "Hwp"; first done.
   iApply step_fupd2N_inner_add.
   iApply (step_fupd2N_inner_wand with "Hwp"); auto.
-  iDestruct 1 as (e2' t2' ?) "(Hσ & Hg & Hwp & Ht & HNC)"; simplify_eq/=.
+  iDestruct 1 as (e2' t2' ?) "(Hσ & Hg & Hwp & Ht)"; simplify_eq/=.
   iMod (fupd2_mask_subseteq ⊤ (⊤ ∖ D)) as "Hclo"; try set_solver+.
-  iMod (NC_upd_C with "HNC") as "#HC".
-  iPoseProof (wpc0_crash with "[$] Hg [$]") as "H".
+  (* iMod (NC_upd_C with "HNC") as "#HC". *)
+  iPoseProof (wpc0_crash with "[$] Hg") as "H".
   iMod "Hclo".
   iDestruct "Hlc2" as "[_ Hlc2]".
   iSpecialize ("H" with "[$]").
   iApply (step_fupd2N_inner_wand _ _ _ _ (S _) with "H"); auto.
   iIntros "(Hg&HΦc)". iNext. iExists _, _. iSplitL ""; first done.
-  iFrame. eauto.
+  iFrame.
 Qed.
 End crash_adequacy.
 
 Section crash_adequacy.
-Context `{!irisGS Λ Σ, generationGS Λ Σ}.
+Context `{!irisGS Λ Σ}.
 Implicit Types s : stuckness.
 Implicit Types e : expr Λ.
 Implicit Types P Q : iProp Σ.
@@ -266,18 +264,16 @@ Lemma wptp_strong_adequacy Φ Φc κs' s n e1 t1 κs t2 σ1 g1 ns mj D σ2 g2 :
   global_state_interp g1 ns mj D (κs ++ κs') -∗
   WPC e1 @ s; ⊤ {{ Φ }} {{ Φc }} -∗
   wptp s t1 -∗
-  NC 1 -∗
   £ (steps_sum num_laters_per_step step_count_next ns n) -∗
   ||={⊤|⊤,∅|∅}=> ||▷=>^(steps_sum num_laters_per_step step_count_next ns n) ||={∅|∅, ⊤|⊤}=> (∃ e2 t2',
     ⌜ t2 = e2 :: t2' ⌝ ∗
     state_interp σ2 (length t2') ∗
     global_state_interp g2 ((Nat.iter n step_count_next ns)) mj D κs' ∗
     from_option Φ True (to_val e2) ∗
-    ([∗ list] v ∈ omap to_val t2', fork_post v) ∗
-    NC 1).
+    ([∗ list] v ∈ omap to_val t2', fork_post v)).
 Proof.
-  iIntros (?) "?? Hwpc Hwptp Hnc Hlc".
-  iApply (wptp0_strong_adequacy mj with "[$] [$] [Hwpc] [Hwptp] [$] [$]"); first eassumption.
+  iIntros (?) "?? Hwpc Hwptp Hlc".
+  iApply (wptp0_strong_adequacy mj with "[$] [$] [Hwpc] [Hwptp] [$]"); first eassumption.
   { by iApply wpc0_wpc. }
   { iApply (big_sepL_mono with "Hwptp"). iIntros.
     iApply (wpc0_wpc); eauto.
@@ -291,14 +287,13 @@ Lemma wptp_progress Φ Φc κs' n e1 t1 κs t2 σ1 g1 ns mj D σ2 g2 e2 :
   global_state_interp g1 ns mj D (κs ++ κs') -∗
   WPC e1 @ NotStuck; ⊤ {{ Φ }} {{ Φc }} -∗
   wptp NotStuck t1 -∗
-  NC 1 -∗
   £ (steps_sum num_laters_per_step step_count_next ns (S n)) -∗
   ||={⊤|⊤,∅|∅}=> ||▷=>^(steps_sum num_laters_per_step step_count_next ns n) ||={∅|∅, ∅|∅}=>
   ||▷=>^(num_laters_per_step (Nat.iter n step_count_next ns) + 1)
   (⌜not_stuck e2 σ2 g2 ⌝).
 Proof.
-  iIntros (??) "?? Hwpc Hwptp Hnc Hlc".
-  iApply (wptp0_progress mj with "[$] [$] [Hwpc] [Hwptp] [$] [$]"); first done; first done.
+  iIntros (??) "?? Hwpc Hwptp Hlc".
+  iApply (wptp0_progress mj with "[$] [$] [Hwpc] [Hwptp] [$]"); first done; first done.
   { by iApply wpc0_wpc. }
   { iApply (big_sepL_mono with "Hwptp"). iIntros.
     iApply (wpc0_wpc); eauto.
@@ -311,15 +306,14 @@ Lemma wptp_strong_crash_adequacy Φ Φc κs' s n e1 t1 κs t2 σ1 g1 ns mj D σ2
   global_state_interp g1 ns mj D (κs ++ κs') -∗
   WPC e1 @ s; ⊤ {{ Φ }} {{ Φc }} -∗
   wptp s t1 -∗
-  NC 1 -∗
   £ (steps_sum num_laters_per_step step_count_next ns (S n)) -∗
   ||={⊤|⊤,∅|∅}=> ||▷=>^(steps_sum num_laters_per_step step_count_next ns (S n)) ||={∅|∅, ⊤|⊤}=>
   ▷ (∃ e2 t2',
     ⌜ t2 = e2 :: t2' ⌝ ∗
-    Φc ∗ state_interp σ2 (length t2') ∗ global_state_interp g2 (Nat.iter n step_count_next ns) mj D κs' ∗ C).
+    Φc ∗ state_interp σ2 (length t2') ∗ global_state_interp g2 (Nat.iter n step_count_next ns) mj D κs').
 Proof.
-  iIntros (?) "?? Hwpc Hwptp Hnc Hlc".
-  iApply (wptp0_strong_crash_adequacy mj with "[$] [$] [Hwpc] [Hwptp] [$] Hlc"); first eassumption.
+  iIntros (?) "?? Hwpc Hwptp Hlc".
+  iApply (wptp0_strong_crash_adequacy mj with "[$] [$] [Hwpc] [Hwptp] Hlc"); first eassumption.
   { by iApply wpc0_wpc. }
   { iApply (big_sepL_mono with "Hwptp"). iIntros.
     iApply (wpc0_wpc); eauto.
